% -------------------------------------------------------------------------------- %

\begin{exercise}

\phantom{}

\begin{align*}
    B(u, v)
    =
    \Int[0][\infty]
    {
        \frac{s^{u-1}}{(1 + s)^{u+v}}
    }{s}
\end{align*}

\end{exercise}

% -------------------------------------------------------------------------------- %

\begin{solution}

\phantom{}

\includegraphicsboxed{Ana3/Ana3 - Gammafunktion & Betafunktion.png}

\begin{align*}
    \implies
    \mathrm{rhs}
    =
    \Int[0][\infty]
    {
        \pbraces
        {
            \frac{s}{s + 1}
        }^{u-1}
        \pbraces
        {
            \frac{1}{s + 1}
        }^{v+1}
    }{s}
    \stackrel{!}{=}
    \Int[0][1]{t^{u-1} (1 - t)^{v-1}}{t}
    =
    \mathrm{lhs}
\end{align*}

Dabei haben wir folgende Substitution verwendet.

\begin{align*}
    t = \frac{s}{s + 1} = \frac{1}{1 + 1/s}
    \implies
    & 1 - t = 1 - \frac{s}{s + 1} = \frac{s + 1 - s}{s + 1} = \frac{1}{s + 1}, \\
    \implies
    & \derivative[][t]{s} = \frac{-1}{(1 + 1/s)^2} \frac{-1}{s^2} = \frac{1}{(s + 1)^2} \implies \mathrm{d}s = \mathrm{d}t (s + 1)^2, \\
    \implies
    & \frac{s}{s + 1} \xrightarrow{s \to \infty} 1
\end{align*}

\end{solution}

% -------------------------------------------------------------------------------- %
