% -------------------------------------------------------------------------------- %

\begin{exercise}[\textbf{Uniform distribution}]

Let $X_1,\dots,X_n$ be a random sample from uniform $(\theta,1)$ distribution,
where $\theta < 1$ is an unknown parameter.

\begin{enumerate}[label = (\alph*)]
  \item Find the MLE $\hat{\theta}$ of $\theta$.
  \item Is $\hat{\theta}$ asymptotically normal? If yes, find the asymptotic
  mean and variance. Otherwise, find a sequence $r_n$ and $a_n$ such that
  $r_n(\hat{\theta} - a_n)$ converges in distribution to a non-degenerate
  (not pointmass) distribution.
\end{enumerate}

\end{exercise}

% -------------------------------------------------------------------------------- %

\begin{solution}

\phantom{}

\begin{enumerate}[label = (\alph*)]
  \item For the maximum likelihood estimation we first determine the
  joint distribution $f_X$.
  \begin{align*}
    L_n(\theta) &= f_X(x_1,\dots,x_n | \theta) 
    = \prod_{i=1}^n f_{X_i}(x_i | \theta)
    = \prod_{i=1}^n \frac{1}{1-\theta}\1_{(\theta,1)}(x_i) \\
    &= \frac{1}{(1-\theta)^n}\1_{(\theta,1)^n}(x_1,\dots,x_n)\\
    &= \begin{cases}
      \frac{1}{(1-\theta)^n}, & \theta < \min_{i=1}^n x_i \\
      0, & \theta \geq \min_{i=1}^n x_i
    \end{cases}.
  \end{align*}

  Clearly, the maximum is attained at the point 
  $\hat{\theta} = \min_{i=1}^n x_i$.

  \item We calculate
  
  \begin{align*}
    F_{\hat{\theta}}(x) &= 1 - \P(\hat{\theta}(X) > x)
    = 1 - \prod_{i=1}^n \frac{(1-x)}{(1-\theta)}
    = 1 - \frac{(1-x)^n}{(1-\theta)^n}
  \end{align*}

  and derive

  \begin{align*}
    f_{\hat{\theta}}(x) = n\frac{(1-x)^{n-1}}{(1-\theta)^{n}}.
  \end{align*}

  

  With the affine transformation $f(x) = r_n(x - a_n)$
  we obtain the distribution

  \begin{align*}
    f_{r_n(\hat{\theta} - a_n)}(y)
    &= f_{\hat{\theta}}(y/r_n + a_n)\frac{1}{r_n} \\
    &= n\frac{(1-y/r_n + a_n)^{n-1}}{(1-\theta)^{n}r_n} \\
    &= \frac{n}{(1- \theta)r_n} \left(\frac{1 - \frac{y}{r_n} - a_n}{1 - \theta}\right)^{n-1}
  \end{align*}

  Setting $r_n = \frac{n - 1}{1 - \theta}$ and $a_n = \theta$ the expression simplifies to
  
  \begin{align*}
    f_{\frac{n - 1}{1 - \theta}(\hat{\theta} - \theta)}(y) &= \frac{n}{n - 1}
    \left(\frac{1 - \theta  - \frac{y(1 - \theta)}{n - 1}}{1 - \theta}\right)^{n-1} \\
    &= \frac{n}{n - 1}\left(1 - \frac{y}{n-1}\right)^{n-1}
    \xrightarrow{n \to \infty} \exp(-y).
  \end{align*}

  Therefore $\frac{n - 1}{1 - \theta}(\hat{\theta} - \theta)$ converges
  in distribution to an exponential distribution with parameter $\lambda = 1$.

\end{enumerate}

\end{solution}

% -------------------------------------------------------------------------------- %
