% -------------------------------------------------------------------------------- %

\begin{exercise}[\textbf{Most powerful test for the normal variance - $\mu$ is unknown}]

    Let $X_1,\dots,X_n$ be i.i.d. $\mathcal{N}(\mu,\sigma^2)$, where $\mu$ is unknown.
    
    
    \begin{enumerate}[label = (\alph*)]
      \item Is there an MP test at level $\alpha$ for testing
      
      \begin{align*}
          H_0: \sigma^2 = \sigma_0^2 \quad \text{vs.} \quad H_1: \sigma^2 = \sigma_1^2, \sigma_1 > \sigma_0?
      \end{align*}

      If not, find the corresponding GLRT.

      \item Is the above generalized likelihood ratio (GLR) test also a GLRT for testing the
      one-sided hypothesis

      \begin{align*}
          H_0: \sigma^2 \leq \sigma_0^2 \quad \text{vs.} \quad H_1: \sigma^2 > \sigma_0^2.
      \end{align*}

      \item Find the GLRT at level $\alpha$ for testing
      
      \begin{align*}
          H_0: \sigma^2 \geq \sigma_0^2 \quad \text{vs.} \quad H_1: \sigma^2 < \sigma_0^2.
      \end{align*}
    \end{enumerate}
    
    \end{exercise}
    
    % -------------------------------------------------------------------------------- %
    
    \begin{solution}
    
    We consider the composite hypotheses $\Theta_0 := \{ (\mu, \sigma_0^2): \mu \in \R\}$
    and $\Theta_1 := \{ (\mu, \sigma_1^2): \mu \in \R \}$.

    \begin{enumerate}[label = (\alph*)]
        \item We already know the general MLE for $(\mu,\sigma^2)$:
        
        \begin{align*}
            \hat{\mu} &= \bar{X} \\
            \hat{\sigma}^2 &= \frac{1}{n}\sum_{i=1}^n (X_i - \bar{X})^2
        \end{align*}

        For the MLE under $H_0$ we simply replace $\hat{\sigma}^2$ by $\sigma_0^2$.

        For the MLE under $H_1$ we simply replace $\hat{\sigma}^2$ by $\sigma_1^2$.

        Now we can write down the GLRT:

        \begin{align*}
            \lambda(\textbf{x}) 
            &= \frac{L(\hat{\mu}, \sigma_1^2 | \textbf{x})}{L(\hat{\mu}, \sigma_0^2 | \textbf{x})} \\
            &= \left(\frac{\sigma_0^2}{\sigma_1^2}\right)^{n/2}
            \exp\left(-\left( \frac{1}{2\sigma_1^2} - \frac{1}{2\sigma_0^2}\right) \sum_{i=1}^n (X_i - \bar{X})^2\right) \\
        \end{align*}
  
        We simplify our test statistic to $T(\textbf{X}) = \sum_{i=1}^n (X_i - \bar{X})^2$.
        Finally we find the corresponding critical value for $T(\textbf{X})$ by solving

        \begin{align*}
            \alpha &\stackrel{!}{=} \sup_{\theta \in \Theta_0} \P(T(\textbf{X}) \geq C) \\
            &= \sup_{\mu \in \R} \P(T(\textbf{X}) \geq C) \\
            &= \sup_{\mu \in \R} \P\left(\sum_{i=1}^n \frac{(X_i - \bar{X})^2}{\sigma_0^2/n} \geq \frac{n}{\sigma_0^2}C\right) \\
            &= 1 - F_{\chi^2(n)}\left(\frac{n}{\sigma_0^2}C\right) \\
            \iff C &= \frac{\sigma_0^2}{n}\chi_{1 - \alpha}^2(n).
        \end{align*}

        \item Our new MLE under $H_0$ for calculating the GLRT for the one-sided
        hypothesis now reads

        \begin{align*}
            \hat{\mu} &= \bar{X} \\
            \hat{\sigma}^2 &= \begin{cases}
                \frac{1}{n}\sum_{i=1}^n (X_i - \bar{X})^2, & \frac{1}{n}\sum_{i=1}^n (X_i - \bar{X})^2 \leq \sigma_0^2 \\
                \sigma_0^2, & \text{otherwise}.
            \end{cases}
        \end{align*}

        Therefore we obtain the new GLR

        \begin{align*}
            \lambda(\textbf{x}) = \begin{cases}
                \left(\frac{\sigma_0^2}{\hat{\sigma}^2}\right)^{n/2}
            \exp\left(-\frac{n}{2}\left(1 - \frac{\hat{\sigma}^2}{\sigma_0^2}\right)\right), & \frac{1}{n}\sum_{i=1}^n (X_i - \bar{X})^2 > \sigma_0^2 \\
            1, & \text{otherwise}.
            \end{cases}
        \end{align*}

        Now we can calculate the critical $C$ by solving

        \begin{align*}
            \alpha \stackrel{!}{=} \sup_{\theta \in \Theta_0}\P(T(\textbf{X}) \geq C)
        \end{align*}
      \end{enumerate}
    
    \end{solution}
    
    % -------------------------------------------------------------------------------- %
    