% --------------------------------------------------------------------------------

\begin{exercise}[The mean of independent normal distributions]

\phantom{}

\begin{enumerate}[label = (\alph*)]

    \item Show that the moment generating function (mgf) of $X \sim \mathcal N(\mu \sigma^2)$ is of the form
    
    \begin{align*}
        M_X(t) = \exp*{\mu t + \frac{\sigma^2 t^2}{2}}.
    \end{align*}

    \item Let $X \sim \mathcal N(\mu, \sigma^2)$ and let $Y = a X + b$ with fixed real constants $a$ and $b$.
    Show that $Y \sim \mathcal N(a \mu + b, a^2 \sigma^2)$.

    \item Let $X_1, \dots, X_n$ be independent identically distributed random variables with $X_1 \sim \mathcal N(\mu, \sigma^2)$.
    Show that the mean $\bar X = \frac{1}{n} (X_1 + \cdots + X_n)$ is also normally distributed and $\bar X \sim \mathcal N(\mu, \frac{\sigma^2}{n})$.

\end{enumerate}

\end{exercise}

% --------------------------------------------------------------------------------

\begin{solution}

\phantom{}

\begin{enumerate}[label = (\alph*)]

    \item

    \begin{align*}
        M_X(t)
        & :=
        E(e^{t x}) \\
        & =
        \Int[-\infty][\infty]
        {
            e^{t x}
            \frac{1}{\sqrt{2 \pi \sigma^2}}
            \exp*{-\frac{(x - \mu)^2}{2 \sigma^2}}
        }{x} \\
        & =
        \frac{1}{\sqrt{2 \pi \sigma^2}}
        \Int[-\infty][\infty]
        {
            \exp*
            {
                t x
                -
                \frac{1}{2} \pbraces{\frac{x - \mu}{\sigma}}^2
            }
        }{x} \\
        & \stackrel{!}{=}
        \frac{1}{\sqrt{2 \pi \sigma^2}}
        \Int[-\infty][\infty]
        {
            \exp*
            {
                t (y \sigma + \mu)
                -
                \frac{y^2}{2}
            }
            \sigma
        }{y} \\
        & =
        \frac{1}{\sqrt{2 \pi}}
        \exp*{\mu t}
        \Int[-\infty][\infty]
        {
            \exp*{-\pbraces{\frac{y^2}{2} - t y \sigma}}
        }{y} \\
        & \stackrel{!!}{=}
        \frac{1}{\sqrt{2 \pi}}
        \exp*{\mu t}
        \Int[-\infty][\infty]
        {
            \exp*
            {
                \frac{(t \sigma)^2}{2}
                -
                \frac{(y - t \sigma)^2}{2}
            }
        }{y} \\
        & \stackrel{!!!}{=}
        \frac{1}{\sqrt{2 \pi}}
        \exp*{\mu t}
        \exp*{\frac{(t \sigma)^2}{2}}
        \underbrace
        {
            \Int[-\infty][\infty]
            {
                \exp*{-\frac{z^2}{2}}
            }{z}
        }_{
            \sqrt{2 \pi}
        }
        \end{align*}

        For \Quote{!} we used

        \begin{align*}
            y = \frac{x - \mu}{\sigma}
            \implies
            \begin{cases}
                x = y \sigma + \mu \\
                \derivative[][y]{x} = \frac{1}{\sigma} \implies \mathrm d x = \sigma \mathrm d y
            \end{cases}.
        \end{align*}

        For \Quote{!!} we used

        \begin{align*}
            \frac{y^2}{2} - t y \sigma
            & =
            \pbraces{\frac{y}{\sqrt 2}}^2 - 2 \frac{y}{\sqrt 2} \frac{t \sigma}{\sqrt 2} + \pbraces{\frac{t \sigma}{\sqrt 2}}^2 - \pbraces{\frac{t \sigma}{\sqrt 2}}^2 \\
            & =
            \pbraces{\frac{y}{\sqrt 2} - \frac{t \sigma}{\sqrt 2}}^2 - \frac{(t \sigma)^2}{2} \\
            & =
            \frac{(y - t \sigma)^2}{2} - \frac{(t \sigma)^2}{2}.
        \end{align*}

        For \Quote{!!!} we used

        \begin{align*}
            z = y - t \sigma
            \implies
            \derivative[][z]{y} = 1
            \implies
            \mathrm d z = \mathrm d y.
        \end{align*}

        \item Consider the linear function
        
        \begin{align*}
            g:
                \R \to \R, \,
                x \mapsto a x + b,
        \end{align*}

        with inverse

        \begin{align*}
            h := g^{-1}:
                \R \to \R, \,
                y \mapsto \frac{y - b}{a},
        \end{align*}

        and Jacobian

        \begin{align*}
            J(y) = h^\prime(y) = \frac{1}{a}.
        \end{align*}

        Note that $Y = g(X)$.
        Recall the Theorem from \cite[Lecture 3, Slide 32]{EStat}.

        \begin{align*}
            f_Y(y)
            =
            f_X(h(y)) |J(y)|
            =
            \frac{1}{\sqrt{2 \pi \sigma^2}}
            \exp*
            {
                -
                \frac
                {
                    \pbraces
                    {
                        \frac{y - b}{a} - \mu
                    }^2
                }{
                    2 \sigma^2
                }
            }
            \frac{1}{|a|}
            =
            \frac{1}{\sqrt{2 \pi (a^2 \sigma^2)}}
            \exp*
            {
                -
                \frac
                {
                    (y - (a \mu + b))^2
                }{
                    2 a^2 \sigma^2
                }
            }
        \end{align*}

        \item According to \href{https://en.wikipedia.org/wiki/Sum_of_normally_distributed_random_variables#:~:text=This%20means%20that%20the%20sum,squares%20of%20the%20standard%20deviations}{Wikipedia},

        \begin{align*}
            X_1                       & \sim \mathcal N(\mu, \sigma^2), \\
            X_1 + X_2                 & \sim \mathcal N(\mu + \mu, \sigma^2 + \sigma^2), \\
            X_1 + X_2 + X_3           & \sim \mathcal N(\mu + \mu + \mu, \sigma^2 + \sigma^2 + \sigma^2), \\
                                      & \, \, \, \vdots \\
            S_n := X_1 + \cdots + X_n & \sim \mathcal N(n \mu, n \sigma^2).
        \end{align*}

        \begin{align*}
            P(\bar X \leq x)
            & =
            P(S_n \leq n x) \\
            & =
            \Int[-\infty][n x]
            {
                \frac{1}{\sqrt{2 \pi n \sigma^2}}
                \exp*
                {
                    -\frac{(\xi - n \mu)^2}{2 n \sigma^2}
                }
            }{\xi} \\
            & \stackrel{!}{=}
            \Int[-\infty][x]
            {
                \frac{1}{\sqrt{2 \pi n \sigma^2}}
                \exp*
                {
                    -\frac{(n \eta - n \mu)^2}{2 n \sigma^2}
                }
                n
            }{\eta} \\
            & =
            \Int[-\infty][x]
            {
                \frac{1}{\sqrt{2 \pi n \sigma^2 / n}}
                \exp*
                {
                    -\frac{(\eta - \mu)^2 n^2}{2 (\sigma^2 / n) n^2}
                }
            }{\eta} \\
            & =
            \Int[-\infty][x]
            {
                \frac{1}{\sqrt{2 \pi \sigma^2 / n}}
                \exp*
                {
                    -\frac{(\eta - \mu)^2}{2 \sigma^2 / n}
                }
            }{\eta}
        \end{align*}

        For \Quote{!} we used

        \begin{align*}
            \eta = \frac{\xi}{n}
            \implies
            \begin{cases}
                \xi = n \eta \\
                \derivative[][\eta]{\xi} = \frac{1}{n} \implies \mathrm d \xi = n \mathrm d \eta
            \end{cases}.
        \end{align*}

\end{enumerate}

\end{solution}

% --------------------------------------------------------------------------------
