\begin{align*}
\begin{array}{ccccc}
    Q_{h_0}^{(1)}(f) = a_{0,0}
    &&&& \\
    & \searrow &&& \\
    Q_{h_1}^{(1)}(f) = a_{1,0}
    & \rightarrow &
    a_{0,1}
    = a_{0,0} + \frac{a_{0,0} - a_{1,0}}{\pbraces{\frac{h_1}{h_0}}^2 - 1}
    && \\
    & \searrow && \searrow & \\
    Q_{h_2}^{(1)}(f) = a_{2,0}
    & \rightarrow &
    a_{1,1}
    = a_{1,0} + \frac{a_{1,0} - a_{2,0}}{\pbraces{\frac{h_2}{h_1}}^2 - 1}
    & \rightarrow &
    a_{0,2}
    = a_{0,1} + \frac{a_{0,1} - a_{1,1}}{\pbraces{\frac{h_2}{h_0}}^2 - 1} \\
\end{array}
\end{align*}