% -------------------------------------------------------------------------------- %

\begin{exercise}[Conditional variance]

\phantom{}
    
\begin{enumerate}[label = (\alph*)]

    \item Show that for any two random variables $X$ and $Y$ the conditional variance identity holds
    
    \begin{align*}
        \Var Y = \E(Var \, (Y \mid X)) + \Var(\E(Y \mid X)),
    \end{align*}

    provided that the expectations exist.
    The law of total expectation (thw tower property) $\E X = \E(\E(Y \mid X))$ should be applied.

    \item Suppose that the distribution of $Y$ conditional on $X = x$ is $\mathcal N (x, x^2)$ and that the marginal distribution of $X$ is uniform on $(0, 1)$.
    Compute $\E Y$ , $\Var Y$ and $\Cov(X, Y)$.

\end{enumerate}

\end{exercise}

% -------------------------------------------------------------------------------- %

\begin{solution}

Conditional variance is just like variance, just replace ordinary expectation with conditional expectation (\cite[Lecture 4, Slide 31]{EStat}).

\begin{align*}
    \Var(Y \mid X)
    & =
    \E \pbraces{(Y - \E(Y \mid X))^2 \mid X} \\
    & =
    \E(Y^2 \mid X) + \E(Y \mid X)^2
\end{align*}

\begin{enumerate}[label = (\alph*)]

    \item We copy the proof from \cite[Lecture 4, Slide 31]{EStat}.
    If $Y$ is integrable, by taking $a(X) = \E Y$ (constant), the law of total expectation and the Conditional Parallel Axis Theorem \cite[Lecture 4, Slide 30]{EStat}, give

    \begin{align*}
        \Var Y
        & =
        \E((Y - \E Y)^2) \\
        & =
        \E((Y - a(X))^2) \\
        & =
        \E(\E((Y - a(X))^2 \mid X)) \\
        & =
        \E(\Var(Y \mid X)) + \E((\E(Y \mid X) - a(X))^2) \\
        & =
        \E(\Var(Y \mid X)) + \E((\E(Y \mid X) - \E Y)^2) \\
        & =
        \E(\Var(Y \mid X)) + \E((\E(Y \mid X) - \E(\E(Y \mid X)))^2) \\
        & =
        \E(\Var(Y \mid X)) + \Var(\E(Y \mid X)),
    \end{align*}

    which obtains the iterated variance formula.

    \item

    \begin{align*}
        \E Y
        & =
        \E(\E(Y \mid X)) \\
        & =
        \E X \\
        & =
        \frac{1}{2}
    \end{align*}

    \begin{align*}
        \E(X^2)
        & =
        \Int[0][1]{x^2}{x} \\
        & =
        \frac{1}{3}
    \end{align*}

    \begin{align*}
        \Var Y
        & =
        \E(\Var(Y \mid X)) + \Var(\E(Y \mid X)) \\
        & =
        \E(X^2) + \Var X \\
        & =
        \frac{1}{3} + \frac{1}{12} \\
        & =
        \frac{5}{12}
    \end{align*}

    \begin{align*}
        \E(X Y)
        & =
        \E(\E(X Y \mid X)) \\
        & =
        \E(X \E(Y \mid X)) \\
        & =
        \E(X^2) \\
        & =
        \frac{1}{3}
    \end{align*}

    \begin{align*}
        \Cov(X, Y)
        & =
        \E(X, Y) - \E X \E Y \\
        & =
        \frac{1}{3} - \frac{1}{2} \frac{1}{2} \\
        & =
        \frac{4}{12} - \frac{3}{12} \\
        & =
        \frac{1}{12}
    \end{align*}

\end{enumerate}

\end{solution}

% -------------------------------------------------------------------------------- %
