% --------------------------------------------------------------------------------

\begin{exercise}[Chi squared distribution]

Let $X$ and $Y$ be independent and identically distributed (i.i.d.) $\mathcal N(0, 1)$ random variables.
Define $Z = \min \Bbraces{X, Y}$.
Show that $Z^2 \sim \chi_1^2$, i.e. show that the pdf of $Z^2$ is given by

\begin{align*}
    f_{Z^2}(z)
    =
    \frac{1}{\sqrt{2 \pi}} \cdot z^{-\frac{1}{2}} \cdot \exp*{-\frac{z}{2}} \cdot \mathbf 1_\Bbraces{z > 0},
\end{align*}

\end{exercise}

% --------------------------------------------------------------------------------

\begin{solution}

\begin{multline*}
    P(Z < z)
    =
    1 - P(Z \geq z)
    =
    1 - P(\min \Bbraces{X, Y} \geq z)
    =
    1 - P(X \geq z, Y \geq z) \\
    =
    1 - P(X \geq z) P(Y \geq z)
    =
    1 - \pbraces{\Int[z][\infty]{\frac{1}{\sqrt{2 \pi}} \exp*{-\frac{\zeta^2}{2}}{\zeta}}{\zeta}}^2
    \stackrel{!}{=}
    1 - \frac{1}{2 \pi} \pbraces{\Int[-\infty][-z]{-\exp*{-\frac{\eta^2}{2}}}{\eta}}^2
\end{multline*}

For \blockquote{!} we used the following substitution and then swapped the integral bounds (the factor $-1$ gets swallowed by the square).

\begin{align*}
    \eta = -\zeta
    \implies
    \begin{cases}
        \derivative[][\eta]{\zeta} = -1 \implies \mathrm d \eta = \mathrm d \zeta \\
        \zeta = -\eta
    \end{cases}
\end{align*}

\begin{align*}
    f_Z(z)
    =
    \derivative{z}
        P(Z < z)
    =
    -\frac{1}{2 \pi}
    \pbraces
    {
        -
        \pbraces
        {
            -\exp*{-\frac{z^2}{2}}
        }
    }
    2
    \Int[-\infty][-z]
    {
        -\exp*{-\frac{\zeta^2}{2}}
    }{\zeta}
    =
    -\frac{1}{\pi}
    \exp*{-\frac{z^2}{2}}
    \Int[-\infty][-z]
    {
        -\exp*{-\frac{\zeta^2}{2}}
    }{\zeta}
\end{align*}

Recall the corollary from \cite[Lecture 3, Slide 42]{EStat}.

\begin{align*}
    \text{lhs}
    & =
    \frac{1}{2 \sqrt z}
    \pbraces
    {
        f_Z(\sqrt z) + f_Z(-\sqrt z)
    }
    \mathbf 1_{(0, \infty)} \\
    & =
    \frac{1}{2 \sqrt z}
    \pbraces
    {
        -
        \frac{1}{\pi}
        \exp*{-\frac{\sqrt z^2}{2}}
        \Int[-\infty][-\sqrt z]
        {
            \exp*{-\frac{\zeta^2}{2}}
        }{\zeta}
        -
        \frac{1}{\pi}
        \exp*{-\frac{(-\sqrt z)^2}{2}}
        \Int[-\infty][-(-\sqrt z)]
        {
            \exp*{-\frac{\zeta^2}{2}}
        }{\zeta}
    }
    \mathbf 1_{(0, \infty)}(z) \\
    & =
    -\frac{1}{2 \sqrt z}
    \frac{1}{\pi}
    \exp*{-\frac{z}{2}}
    \pbraces
    {
        \Int[-\infty][-\sqrt z]
        {
            -\exp*{-\frac{\zeta^2}{2}}
        }{\zeta}
        +
        \Int[-\sqrt z][\infty]
        {
            -\exp*{-\frac{\zeta^2}{2}}
        }{\zeta}
    }
    \mathbf 1_{(0, \infty)}(z) \\
    & =
    \frac{1}{2 \pi}
    z^{-\frac{1}{2}}
    \exp*{-\frac{z}{2}}
    \underbrace
    {
        \Int[-\infty][\infty]
        {
            \exp*{-\frac{\zeta^2}{2}}
        }{\zeta}
    }_{
        \sqrt{2 \pi}
    }
    \mathbf 1_{(0, \infty)}(z) \\
    & =
    \text{rhs}
\end{align*}

\end{solution}

% --------------------------------------------------------------------------------
