% -------------------------------------------------------------------------------- %

\begin{exercise}

Benützen Sie das vorherige Beispiel um zu zeigen, dass die einzigen
Lösungen von $x^2 + y^2 = z^2$ mit $(x,y) = 1$ und $x \equiv 0 \mod{2}$
gegeben sind durch

\begin{align*}
    x = 2ab, \quad y = a^2 - b^2 \quad \text{und } z = a^2 + b^2, 
\end{align*}

wobei $a,b \in \Z$ mit $(a,b) = 1$.

\textit{Hinweis:} $x^2 + y^2 = (x + iy)(x - iy)$.

\end{exercise}

% -------------------------------------------------------------------------------- %

\begin{solution}

\phantom{}

\end{solution}

% -------------------------------------------------------------------------------- %
