% --------------------------------------------------------------------------------

\begin{exercise}

Zeigen Sie dass $\Bbraces{ab, aba}^\ast = \Bbraces{\epsilon} \cup \Bbraces{a} \Bbraces{ba, baa}^\ast \Bbraces{b, ba}$.

\end{exercise}

% --------------------------------------------------------------------------------

\begin{solution}

Sei $L$ die linke und $R$ die rechte Menge.

\begin{enumerate}[label = \arabic*.]

    \item Inklusion ($L \subseteq R$):
    
    Wir verwenden Induktion nach $k \geq 0$, um zu zeigen, dass

    \begin{align*}
        L = \bigcup_{k \geq 0} \Bbraces{ab, aba}^k \subseteq R.
    \end{align*}

    \begin{itemize}

        \item ($k = 0$):
        
        \begin{align*}
            \Bbraces{ab, aba}^0
            =
            \Bbraces{\epsilon}
            \subseteq
            R
        \end{align*}

        \item ($k = 1$):
        
        \begin{align*}
            \Bbraces{ab, aba}^1
            =
            \Bbraces{ab, aba} \Bbraces{\epsilon}
            =
            \Bbraces{a} \Bbraces{b, ba}
            \subseteq
            R
        \end{align*}

        \item ($k \mapsto k + 1$):
        
        \begin{align*}
            \Bbraces{ab, aba}^{k+1}
            & =
            \Bbraces{ab, aba} \Bbraces{ab, aba}^k \\
            & \subseteq^\text{IH}
            \Bbraces{ab, aba} R \\
            & =
            \Bbraces{ab, aba} \Bbraces{\epsilon} \cup \Bbraces{ab, aba} \Bbraces{a} \Bbraces{ba, baa}^\ast \Bbraces{b, ba} \\
            & =
            \Bbraces{ab, aba}^1 \cup \Bbraces{a} \Bbraces{ba, baa}^\ast \Bbraces{b, ba} \\
            & \subseteq
            R \cup R
            =
            R
        \end{align*}

    \end{itemize}

    \item Inklusion ($R \subseteq L$):
    
    FÃ¼r $k = 0$ sieht man $\Bbraces{\epsilon} \subseteq L$.
    Wir verwenden Induktion nach $k \geq 0$, um zu zeigen, dass

    \begin{align*}
        R
        =
        \Bbraces{\epsilon} \cup \Bbraces{a} \pbraces{\bigcup_{k \geq 0} \Bbraces{ba, baa^k}} \Bbraces{b, ba}
        =
        \Bbraces{\epsilon} \cup \bigcup_{k \geq 0} \Bbraces{a} \Bbraces{ba, baa}^k \Bbraces{b, ba}
        \subseteq
        L.
    \end{align*}

    \begin{itemize}
        \item ($k = 0$):
        
        \begin{align*}
            \Bbraces{a} \Bbraces{ba, baa}^0 \Bbraces{b, ba}
            =
            \Bbraces{a} \Bbraces{\epsilon} \Bbraces{b, ba}
            =
            \Bbraces{ab, aba}
            \subseteq
            L
        \end{align*}

        \item ($k \mapsto k + 1$):
        
        \begin{align*}
            \Bbraces{a} \Bbraces{ba, baa}^{k+1} \Bbraces{b, ba}
            & =
            \Bbraces{a} \Bbraces{ba, baa}^k \Bbraces{ba, baa} \Bbraces{b, ba} \\
            & =
            \Bbraces{a} \Bbraces{ba, baa}^k \Bbraces{b, ba} \Bbraces{a} \Bbraces{b, ba} \\
            & \subseteq^\text{IH}
            \Bbraces{ab, aba}^\ast \Bbraces{ab, aba} \\
            & =
            \Bbraces{ab, aba}^+ \\
            & \subseteq
            L
        \end{align*}

    \end{itemize}

\end{enumerate}

\end{solution}

% --------------------------------------------------------------------------------
