% --------------------------------------------------------------------------------

\begin{exercise}[\textbf{Minimal sufficient statistic 1}]

Let $X_1,\dots,X_n$ be a random sample from a population with $\mathcal{N}(\mu,\mu)$
distribution, where $\mu > 0$ is unknown.

\begin{enumerate}[label = (\alph*)]
  \item Show that the statistic $\sum_{i=1}^n X_i^2$ is minimal sufficient
  in the $\mathcal{N}(\mu,\mu)$ family.
  \item Show that the statistic $\left(\sum_{i=1}^n X_i, \sum_{i=1}^n X_i^2\right)$ is sufficient
  but not minimal sufficient in the $\mathcal{N}(\mu,\mu)$ family.
\end{enumerate}

\end{exercise}

% --------------------------------------------------------------------------------

\begin{solution}

  \phantom{}

  \begin{enumerate}[label = (\alph*)]
    \item 
    First we calculate the joint pdf:
    \begin{align*}
      f(\textbf{x}|\mu) = \frac{1}{(2\pi\mu)^{n/2}}
      \exp\left(-\frac{1}{2\mu}\sum_{i=1}^n(x_i - \mu)^2\right)
    \end{align*}
    Let $\textbf{x} = (x_1,\dots,x_n)$ and $\textbf{y} = (y_1,\dots,y_n)$ 
    be two sample points. We calculate the ratio

    \begin{align*}
      \frac{f(\textbf{x}|\mu)}{f(\textbf{y}|\mu)}
      &= \frac{\exp\left(-\frac{1}{2\mu}\sum_{i=1}^n(x_i - \mu)^2\right)}
            {\exp\left(-\frac{1}{2\mu}\sum_{i=1}^n(y_i - \mu)^2\right)} \\
      &= \exp\left(-\frac{1}{2\mu}\sum_{i=1}^n[(x_i - \mu)^2 - (y_i - \mu)^2]\right) \\
      &= \exp\left(-\frac{1}{2\mu}\sum_{i=1}^n [x_i^2 - 2\mu x + \mu^2 - y_i^2 + 2\mu y - \mu^2]\right) \\
      &= \exp\left(-\frac{1}{2\mu}\sum_{i=1}^n [x_i^2 - y_i^2] + \sum_{i=1}^n [y_i - x_i]\right), \\
    \end{align*}

    which is constant as a function of $\mu$ if and only if $\sum_{i=1}^n x_i^2 = \sum_{i=1}^n y_i^2$.

    Therefore $T(\textbf{x}) = \sum_{i=1}^n x_i^2$ is a minimal sufficient statistic for estimating $\mu$.

    \item Factorizing the joint pdf into
    
    \begin{align*}
      f(\textbf{x}|\mu) &= \exp\left(-\frac{1}{2\mu}\sum_{i=1}^n(x_i - \mu)^2\right) \\
      &= \exp\left(-\frac{1}{2\mu}\sum_{i=1}^n(x_i^2 - 2\mu x_i + \mu^2\right) \\
      &= \exp\left(-\frac{1}{2\mu}\left(\sum_{i=1}^n x_i^2\right) + \sum_{i=1}^n x_i - 2n\mu\right) =: g(T(x)|\theta) \cdot 1
    \end{align*}
    
    we can clearly see that $T(X) = \left(\sum_{i=1}^n X_i, \sum_{i=1}^n X_i^2\right)$ is a sufficient statistic.
    
    Since there is no function $r$ such that 

    \begin{align*}
      r\left(\sum_{i=1}^n X_i^2\right) = \left(\sum_{i=1}^n X_i, \sum_{i=1}^n X_i^2\right).
    \end{align*}

    and $\sum_{i=1}^n X_i^2$ is a (minimal) sufficient statistic, this means by definition
    $\left(\sum_{i=1}^n X_i, \sum_{i=1}^n X_i^2\right)$ cannot be minimal sufficient.
  \end{enumerate}

\end{solution}

% --------------------------------------------------------------------------------
