% --------------------------------------------------------------------------------

\begin{exercise}

Bestimmen Sie die Fouriertransformierte der Funktion

\begin{align*}
    f(x)
    =
    \frac{1}{1 + x + x^2}.
\end{align*}

\end{exercise}

% --------------------------------------------------------------------------------

\begin{solution}

\begin{align*}
    g(t) := e^{-\lambda |t|},
    \quad
    t \in \R,
    \quad
    \lambda > 0
\end{align*}

\begin{align*}
    g^\wedge(t)
    & =
    \frac{1}{\sqrt{2 \pi}}
    \Int[\R]
    {
        e^{-i t x}
        e^{-\lambda |x|}
    }{x} \\
    & =
    \frac{1}{\sqrt{2 \pi}}
    \pbraces
    {
        \Int[-\infty][0]
        {
            e^{-i t x}
            e^{\lambda x}
        }{x}
        +
        \Int[0][\infty]
        {
            e^{-i t x}
            e^{-\lambda x}
        }{x}    
    } \\
    & =
    \frac{1}{\sqrt{2 \pi}}
    \pbraces
    {
        \Int[-\infty][0]
        {
            e^{(\lambda - i t) x}
        }{x}
        +
        \Int[0][\infty]
        {
            e^{(\lambda + i t) x}
        }{x}
    } \\
    & =
    \frac{1}{\sqrt{2 \pi}}
    \Bigg (
        \frac{1}{\lambda - i t}
        \underbrace
        {
            e^{(\lambda - i t) x} \Big |_{x = -\infty}^0
        }_1
        +
        \frac{1}{\lambda + i t}
        \underbrace
        {
            e^{(\lambda + i t) x} \Big |_{x=0}^\infty
        }_1
    \Bigg ) \\
    & =
    \frac{1}{\sqrt{2 \pi}}
    \pbraces
    {
        \frac{1}{\lambda - i t}
        +
        \frac{1}{\lambda + i t}
    } \\
    & =
    \frac{1}{\sqrt{2 \pi}}
    \frac
    {
        (\lambda + i t)
        +
        (\lambda - i t)
    }{
        (\lambda - i t)
        (\lambda + i t)
    } \\
    & =
    \frac{1}{\sqrt{2 \pi}}
    \frac{2 \lambda}{t^2 + \lambda^2} \\
    & =
    \sqrt \frac{2}{\pi}
    \frac{1}{t^2 + \lambda^2}
\end{align*}

\begin{align*}
    & \implies
    h_\lambda(t)
    :=
    \frac{1}{t^2 + \lambda^2}
    =
    \sqrt \frac{\pi}{2}
    g^\wedge(t) \\
    & \implies
    h_\lambda^\wedge(t)
    =
    \sqrt \frac{\pi}{2}
    g(t)
    =
    \sqrt \frac{\pi}{2}
    e^{-\lambda |t|}
\end{align*}

\begin{align*}
    \lambda := \sqrt{\frac{3}{4}}
    \implies
    f^\wedge(t)
    & =
    \frac{1}{\sqrt{2 \pi}}
    \Int[\R]
    {
        e^{-i t x}
        f(x)
    }{x} \\
    & =
    \frac{1}{\sqrt{2 \pi}}
    \Int[\R]
    {
        e^{-i t x}
        \frac{1}{1 + x + x^2}
    }{x} \\
    & =
    \frac{1}{\sqrt{2 \pi}}
    \Int[\R]
    {
        e^{-i t \pbraces{x + \frac{1}{2}}}
        e^{i t \frac{1}{2}}
        \frac{1}
        {
            \pbraces{\frac{1}{2}}^2
            +
            2 x \frac{1}{2}
            +
            x^2
            +
            \frac{3}{4}
        }
    }{x} \\
    & =
    \frac{1}{\sqrt{2 \pi}}
    e^{i t \frac{1}{2}}
    \Int[\R]
    {
        e^{-i t \pbraces{x + \frac{1}{2}}}
        \frac{1}
        {
            \pbraces
            {
                \frac{1}{2}
                +
                x
            }^2
            +
            \frac{3}{4}
        }
    }{x} \\
    & =
    \frac{1}{\sqrt{2 \pi}}
    e^{i t \frac{1}{2}}
    \Int[\R]
    {
        e^{-i t u}
        \frac{1}
        {
            u^2
            +
            \lambda^2
        }
    }{u} \\
    & =
    \frac{1}{\sqrt{2 \pi}}
    e^{i t \frac{1}{2}}
    h_\lambda^\wedge(t) \\
    & =
    \frac{1}{\sqrt{2 \pi}}
    e^{i t \frac{1}{2}}
    \sqrt \frac{\pi}{2}
    e^{-\lambda |t|} \\
    & =
    \frac{1}{2}
    e^{
        i t \frac{1}{2}
        -
        \sqrt{\frac{3}{4}} |t|
    }
\end{align*}

\end{solution}

% --------------------------------------------------------------------------------
