\begin{align*}
    Q_{h_1}^{(1)}(f)
    & = \frac{h_1}{2}
        \pbraces
        {
            f(a) +
            2 \sum_{i=1}^{n_1 - 1} f(y_i) +
            f(b)
        } \\
    & = \frac{h_0}{4}
        \pbraces
        {
            f(a) +
            2 \sum_{i=1}^{2 n_0 - 1} f(y_i) +
            f(b)
        } \\
    & = \frac{h_0}{4}
        \pbraces
        {
            f(a) +
            2 \pbraces
            {
                \sum_{i=1}^{n_0 - 1} f(y_{2i}) +
                \sum_{i=1}^{n_0} f(y_{2i-1})
            }
            f(b)
        } \\
    & = \frac{h_0}{4}
        \pbraces
        {
            f(a) +
            2 \pbraces
            {
                \sum_{i=1}^{n_0 - 1} f(x_i) +
                \sum_{i=1}^{n_0} f \pbraces{\frac{x_{i-1} - x_i}{2}}
            } +
            f(b)
        } \\
    & = \frac{1}{2}
        \pbraces
        {
            \frac{h_0}{2}
            \pbraces
            {
            f(a) +
            2 \sum_{i=1}^{n_0 - 1} f(x_i) +
            f(b)
            } +
            h_0 \sum_{i=1}^{n_0} f \pbraces{\frac{x_{i-1} - x_i}{2}}
        } \\
    & = \frac{1}{2}
        \pbraces
        {
            Q_{h_0}^{(1)}(f) +
            h_0 \sum_{i=1}^{n_0} f \pbraces{\frac{x_{i-1} - x_i}{2}}
        }
    \label{effiziente_extrapolation}
\end{align*}