\begin{align*}
    a_{0,1}
    & = Q_{h_0}^{(1)}(f) +
        \frac
        {Q_{h_0}^{(1)}(f) - Q_{h_1}^{(1)}(f)}
        {\pbraces{\frac{1}{2}}^2 - 1} \\
    & = \frac{1}{3}
        \pbraces
        {
            - Q_{h_0}^{(1)}(f)
            + 4 Q_{h_1}^{(1)}(f)
        } \\
    & = \frac{1}{3}
        \pbraces
        {
            - \frac{h_0}{2}
            \pbraces
            {
                f(a) +
                2 \sum_{i=1}^{n_0 - 1} f(x_i) +
                f(b)
            }
            + 4 \frac{h_1}{2}
            \pbraces
            {
                f(a) +
                2 \sum_{i=1}^{n_1 - 1} f(y_i) +
                f(b)
            }
        } \\
    & = \frac{1}{3}
        \pbraces
        {
            - \frac{h_0}{2}
            \pbraces
            {
                f(a) +
                2 \sum_{i=1}^{n_0 - 1} f(x_i) +
                f(b)
            }
            + \frac{2 h_0}{2}
            \pbraces
            {
                f(a) +
                2 \sum_{i=1}^{2 n_0 - 1} f(y_i) +
                f(b)
            }
        } \\
    & = \frac{h_0}{3}
        \pbraces
        {
            - \frac{1}{2}
            \pbraces
            {
                f(a) +
                2 \sum_{i=1}^{n_0 - 1} f(x_i) +
                f(b)
            }
            + \pbraces
            {
                f(a) +
                2 \pbraces
                {
                    \sum_{i=1}^{n_0} f(y_{2i-1}) +
                    \sum_{i=1}^{n_0-1} f(y_{2i})
                } +
                f(b)
            }
        } \\
    & = \frac{h_0}{3}
        \pbraces
        {
            - \frac{1}{2}
            \pbraces
            {
                f(a) +
                2 \sum_{i=1}^{n_0 - 1} f(x_i) +
                f(b)
            }
            + \pbraces
            {
                f(a) +
                2 \pbraces
                {
                    \sum_{i=1}^{n_0}
                    f \pbraces{\frac{x_{i-1} - x_i}{2}} +
                    \sum_{i=1}^{n_0-1} f(x_i)
                } +
                f(b)
            }
        } \\
    & = \frac{h_0}{6}
        \pbraces
        {
            f(a) +
            4 \sum_{i=1}^{n_0}
            f \pbraces{\frac{x_{i-1} - x_i}{2}} +
            2 \sum_{i=1}^{n_0 - 1} f(x_i) +
            f(b)
        } \\
    & = Q_{h_0}^{(2)}(f)
\end{align*}