\begin{align*}
    & a_{0,2} \\
    & = Q_{h_0}^{(2)}(f) +
        \frac
        {Q_{h_0}^{(2)}(f) - Q_{h_1}^{(2)}(f)}
        {\pbraces{\frac{1}{2^2}}^2 - 1} \\
    & = \frac{1}{15}
        \pbraces
        {
            - Q_{h_0}^{(2)}(f)
            + 16 Q_{h_1}^{(2)}(f)
        } \\
    & = \frac{1}{15}
        \Bigg (
            - \frac{h_0}{6}
            \pbraces
            {
                f(a) +
                2 \sum_{i=1}^{n_0 - 1} f(x_i) +
                4 \sum_{i=1}^{n_0} f \pbraces{\frac{x_{i-1} + x_i}{2}} +
                f(b)
            } \\
    & +
            16 \frac{h_1}{6}
            \pbraces
            {
                f(a) +
                2 \sum_{i=1}^{n_1 - 1} f(y_i) +
                4 \sum_{i=1}^{n_1} f \pbraces{\frac{y_{i-1} + y_i}{2}} +
                f(b)
            }
        \Bigg ) \\
    & = \frac{1}{15}
        \Bigg (
            - \frac{h_0}{6}
            \pbraces
            {
                f(a) +
                2 \sum_{i=1}^{n_0 - 1} f(x_i) +
                4 \sum_{i=1}^{n_0} f \pbraces{\frac{x_{i-1} + x_i}{2}} +
                f(b)
            } \\
    & +
            \frac{8 h_0}{6}
            \pbraces
            {
                f(a) +
                2 \sum_{i=1}^{2 n_0 - 1} f(y_i) +
                4 \sum_{i=1}^{2 n_0} f \pbraces{\frac{y_{i-1} + y_i}{2}} +
                f(b)
            }
        \Bigg ) \\
    & = \frac{h_0}{90}
        \Bigg (
            - \pbraces
            {
                f(a) +
                2 \sum_{i=1}^{n_0 - 1} f(x_i) +
                4 \sum_{i=1}^{n_0} f \pbraces{\frac{x_{i-1} + x_i}{2}} +
                f(b)
            } \\
    & +
            8 \pbraces
            {
                f(a) +
                2 \pbraces
                {
                    \sum_{i=1}^{n_0} f(y_{2i-1}) +
                    \sum_{i=1}^{n_0 - 1} f(y_{2i})
                } +
                4 \pbraces
                {
                    \sum_{i=1}^{n_0} f \pbraces{\frac{y_{2i-2} + y_{2i-1}}{2}} +
                    \sum_{i=1}^{n_0} f \pbraces{\frac{y_{2i-1} + y_{2i}}{2}}
                } +
                f(b)
            }
        \Bigg ) \\
    & = \frac{h_0}{90}
        \Bigg (
            - \pbraces
            {
                f(a) +
                2 \sum_{i=1}^{n_0 - 1} f(x_i) +
                4 \sum_{i=1}^{n_0} f \pbraces{\frac{x_{i-1} + x_i}{2}} +
                f(b)
            } \\
    & +
            8 \pbraces
            {
                f(a) +
                2 \pbraces
                {
                    \sum_{i=1}^{n_0} f \pbraces{\frac{x_{i-1} - x_i}{2}} +
                    \sum_{i=1}^{n_0 - 1} f(x_i)
                } +
                4 \pbraces
                {
                    \sum_{i=1}^{n_0} f \pbraces{\frac{3 x_{i-1} + x_i}{4}} +
                    \sum_{i=1}^{n_0} f \pbraces{\frac{x_{i-1} + 3 x_i}{4}}
                } +
                f(b)
            }
        \Bigg ) \\
    & = \frac{h_0}{90}
        \Bigg (
            - \pbraces
            {
                f(a) +
                2 \sum_{i=1}^{n_0 - 1} f(x_i) +
                4 \sum_{i=1}^{n_0} f \pbraces{\frac{x_{i-1} + x_i}{2}} +
                f(b)
            } \\
    & +
            8 \pbraces
            {
                f(a) +
                2 \pbraces
                {
                    \sum_{i=1}^{n_0} f \pbraces{\frac{x_{i-1} - x_i}{2}} +
                    \sum_{i=1}^{n_0 - 1} f(x_i)
                } +
                4 \pbraces
                {
                    \sum_{i=1}^{n_0} f \pbraces{\frac{3 x_{i-1} + x_i}{4}} +
                    \sum_{i=1}^{n_0} f \pbraces{\frac{x_{i-1} + 3 x_i}{4}}
                } +
                f(b)
            }
        \Bigg ) \\
    & = \frac{h_0}{90}
        \pbraces
        {
            7 f(a) +
            32 \sum_{i=1}^{n_0} f \pbraces{\frac{3 x_{i-1} + x_i}{4}} +
            12 \sum_{i=1}^{n_0} f \pbraces{\frac{x_{i-1} + x_i}{2}} +
            14 \sum_{i=1}^{n_0 - 1} f(x_i) +
            32 \sum_{i=1}^{n_0} f \pbraces{\frac{x_{i-1} + 3 x_i}{4}} +
            7 f(b)
        } \\
    & = Q_{h_0}^{(4)}(f)
\end{align*}