% --------------------------------------------------------------------------------

\begin{exercise}[Card game]

A deck of $52$ cards has $13$ ranks ($2$, $3$, $4$, $5$, $6$, $7$, $8$, $9$, $10$, $J$, $Q$, $K$, $A$) an $4$ suits ($\textcolor{red}{\heartsuit}$, $\spadesuit$, $\textcolor{red}{\diamondsuit}$, $\clubsuit$).
Three cards are drawn randomly without replacement from a deck of $52$ cards.

\begin{enumerate}[label = (\alph*)]
    \item What ist the probability that all cards are in the same suit?
    \item What ist the probability that all cards have the same rank?
    \item What ist the probability that the three cards contain exactly one pair (a pair means two cards with the same rank from two different suits)?
\end{enumerate}

\end{exercise}

% --------------------------------------------------------------------------------

\begin{solution}

Let $X_i$ denote the card that gets chosen in the $i$-th step and

\begin{align*}
    S := \Bbraces{\textcolor{red}{\heartsuit}, \spadesuit, \textcolor{red}{\diamondsuit}, \clubsuit},
    \quad
    R := \Bbraces{2, 3, 4, 5, 6, 7, 8, 9, 10, J, Q, K, A}
\end{align*}

\begin{enumerate}[label = (\alph*)]

    \item

    \begin{align*}
        &
        P(\operatorname{suit} X_1 = \cdots = \operatorname{suit} X_3) \\
        & =
        \sum_{s \in S} P(\operatorname{suit} X_1 = \cdots = \operatorname{suit} X_3 = s) \\
        & =
        \sum_{s \in S} P(\operatorname{suit} X_1 = s) P(\operatorname{suit} X_2 = s \mid \operatorname{suit} X_1 = s) P(\operatorname{suit} X_3 = s \mid \operatorname{suit} X_1 = \operatorname{suit} X_2 = s) \\
        & =
        |S| \frac{13}{52} \frac{12}{51} \frac{11}{50}
    \end{align*}

    \item

    \begin{align*}
        &
        P(\operatorname{rank} X_1 = \dots = \operatorname{rank} X_3) \\
        & =
        \sum_{r \in R} P(\operatorname{rank} X_1 = \cdots = \operatorname{rank} X_3 = r) \\
        & =
        \sum_{r \in R} P(\operatorname{rank} X_1 = r) P(\operatorname{rank} X_2 = r \mid \operatorname{rank} X_1 = r) P(\operatorname{rank} X_3 = r \mid \operatorname{rank} X_1 = \operatorname{rank} X_2 = r) \\
        & =
        |R| \frac{4}{52} \frac{3}{51} \frac{2}{50}
    \end{align*}

    \item

    \begin{align*}
        &
        P((X_1, \dots, X_3) ~\text{contains exactly one pair}) \\
        & =
        P(|\Bbraces{\operatorname{rank} X_1, \dots, \operatorname{rank} X_3}| = 2) \\
        & =
        P(\operatorname{rank} X_1 = \operatorname{rank} X_2 \neq \operatorname{rank} X_3) \\
        & +
        P(\operatorname{rank} X_2 = \operatorname{rank} X_3 \neq \operatorname{rank} X_1) \\
        & +
        P(\operatorname{rank} X_3 = \operatorname{rank} X_1 \neq \operatorname{rank} X_2) \\
        & =
        \sum_{r_1 \in R} \sum_{r_2 \in R \setminus \Bbraces{r_1}}
            P(\operatorname{rank} X_1 = \operatorname{rank} X_2 = r_1, \operatorname{rank} X_3 = r_2) \\
        & +
        \sum_{r_1 \in R} \sum_{r_2 \in R \setminus \Bbraces{r_1}}
            P(\operatorname{rank} X_2 = \operatorname{rank} X_3 = r_2, \operatorname{rank} X_1 = r_1) \\
        & +
        \sum_{r_1 \in R} \sum_{r_2 \in R \setminus \Bbraces{r_1}}
            P(\operatorname{rank} X_3 = \operatorname{rank} X_1 = r_1, \operatorname{rank} X_2 = r_2) \\
        & =
        \sum_{r_1 \in R} \sum_{r_2 \in R \setminus \Bbraces{r_1}} \\
            & P(\operatorname{rank} X_1 = r_1) P(\operatorname{rank} X_2 = r_1 \mid \operatorname{rank} X_1 = r_1) P(\operatorname{rank} X_3 = r_2 \mid \operatorname{rank} X_1 = r_1, \operatorname{rank} X_2 = r_1)
            + \\
            & P(\operatorname{rank} X_1 = r_1) P(\operatorname{rank} X_2 = r_2 \mid \operatorname{rank} X_1 = r_1) P(\operatorname{rank} X_3 = r_2 \mid \operatorname{rank} X_1 = r_1, \operatorname{rank} X_2 = r_2)
            + \\
            & P(\operatorname{rank} X_1 = r_2) P(\operatorname{rank} X_2 = r_2 \mid \operatorname{rank} X_1 = r_1) P(\operatorname{rank} X_3 = r_2 \mid \operatorname{rank} X_1 = r_1, \operatorname{rank} X_2 = r_2) \\
        & =
        |R| (|R| - 1)
        \pbraces
        {
            \frac{4}{52} \frac{3}{51} \frac{12 \cdot 4}{50}
            +
            \frac{4}{52} \frac{12 \cdot 4}{51} \frac{12 \cdot 4 - 1}{50}
            +
            \frac{4}{52} \frac{12 \cdot 4}{51} \frac{3}{50}
        } \\
    	& =
    	13 \cdot 12 \frac{1}{13} 
    	\pbraces
    	{
    		\frac{3}{51} \frac{12 \cdot 4}{50}
    		+
    		\frac{12 \cdot 4}{51} \frac{12 \cdot 4 - 1}{50}
    		+
    		\frac{12 \cdot 4}{51} \frac{3}{50}
    	} \\
    	& = 12 \frac{3 \cdot 48 + 48 \cdot 47 + 48 \cdot 3 }{50 \cdot 51} = 4 \cdot 24 \frac{3 + 47 + 3}{25 \cdot 17} = \frac{53 \cdot 96}{25 \cdot 17} > 1
    \end{align*}

\end{enumerate}

\end{solution}

% --------------------------------------------------------------------------------
