% --------------------------------------------------------------------------------

\begin{exercise}[Independence]

Let $A$ and $B$ be two independent events.

\begin{enumerate}[label = (\alph*)]

    \item Prove that $A^c$ and $B^c$ are also independent.

    \item If we additionally know that $P(A | B) = 0.6$ and $P(B | A) = 0.3$, compute the probabilities of the following two events

    \begin{enumerate}[label = (\roman*)]
        \item at most one of $A$ or $B$
        \item either $A$ or $B$ but not both.
    \end{enumerate}

\end{enumerate}

\end{exercise}

% --------------------------------------------------------------------------------

\begin{solution}

\phantom{}

\begin{enumerate}[label = (\alph*)]

    \item

    \begin{multline*}
        P(A^c \cap B^c)
        =
        P((A \cup B)^c)
        =
        1 - P(A \cup B)
        =
        1 - (P(A) + P(B) - P(A \cap B)) \\
        =
        1 - P(A) - P(B) + P(A) P(B)
        =
        (1 - P(A)) (1 - P(B))
        =
        P(A^c) P(B^c)
    \end{multline*}

    \item

    \begin{align*}
        &
        P(A ~|~ B) = \frac{P(A \cap B)}{P(B)},
        \quad
        P(B ~|~ A) = \frac{P(B \cap A)}{P(A)} \\
        & \implies
        P(A) P(B)
        =
        P(A \cap B)
        =
        \begin{cases}
            P(A ~|~ B) P(B) \\
            P(B ~|~ A) P(A)
        \end{cases} \\
        & \implies
        P(A) = P(A ~|~ B) = \frac{6}{10},
        \quad
        P(B) = P(B ~|~ A) = \frac{3}{10}
    \end{align*}

    \begin{enumerate}[label = (\roman*)]

        \item

        \begin{multline*}
            P(A^c \cap B^c) + P(A^c \cap B) + P(A \cap B^c)
            =
            1 - P(A \cap B)
            =
            1 - P(A) P(B)
            =
            1 - \frac{6}{10} \frac{3}{10} \\
            =
            1 - \frac{18}{100}
            =
            \frac{41}{100}
        \end{multline*}

        \item

        \begin{multline*}
            P(A \Delta B)
            =
            P(A) P(B^c) + P(A^c) P(B)
            =
            P(A) (1 - P(B)) + (1 - P(A)) P(B) \\
            =
            \frac{6}{10} \pbraces{1 - \frac{3}{10}} + \pbraces{1 - \frac{6}{10}} \frac{3}{10}
            =
            \frac{6}{10} \frac{7}{10} + \frac{4}{10} \frac{3}{10}
            =
            \frac{42}{100} + \frac{12}{100}
            =
            \frac{54}{100}
            =
            \frac{27}{100}
        \end{multline*}

    \end{enumerate}

\end{enumerate}

\end{solution}

% --------------------------------------------------------------------------------
