% --------------------------------------------------------------------------------

\begin{exercise}[Box with coins]

A box contains three coins with a head on each side, two coins with a tail on each side, and four fair coins.

\begin{enumerate}[label = (\alph*)]

    \item One of these nine coins is selected at random and tossed once.
    What is the probability of getting a tail?

    \item If we get a tail, what is the probability that the selected coin has a tail on both side?
    If we get a tail, what is the probability that it is a fair coin?

    \item If the first toss is tail, and another coin is selected at random from the remaining eight coins and tossed once, what is the probability of getting a tail again?

\end{enumerate}

\end{exercise}

% --------------------------------------------------------------------------------

\begin{solution}

Let $X_i$ denote the type of the $i$-th selected coin (head, tail, or fair) and $Y_i$ the yield of the $i$-th toss (head or tail).
Furthermore, to ease notation, let $X := X_1$ and $Y := Y_1$.

\begin{enumerate}[label = (\alph*)]

    \item

    \begin{align*}
        P(Y = \mathrm{tail})
        & =
        P(Y = \mathrm{tail} \mid X = \mathrm{head}) P(X = \mathrm{head}) \\
        & +
        P(Y = \mathrm{tail} \mid X = \mathrm{tail}) P(X = \mathrm{tail}) \\
        & +
        P(Y = \mathrm{tail} \mid X = \mathrm{fair}) P(X = \mathrm{fair}) \\
        & =
        0 \frac{3}{3 + 2 + 4} + 1 \frac{2}{3 + 2 + 4} + \frac{1}{2} \frac{4}{3 + 2 + 4} \\
        & =
        \frac{4}{9}
    \end{align*}

    \item

    \begin{multline*}
        P(X = \mathrm{tail} \mid Y = \mathrm{tail})
        =
        \frac{P(X = \mathrm{tail}, Y = \mathrm{tail})}{P(Y = \mathrm{tail})}
        =
        \frac{P(Y = \mathrm{tail} \mid X = \mathrm{tail}) P(X = \mathrm{tail})}{P(Y = \mathrm{tail})} \\
        =
        \frac{1 \frac{2}{3 + 2 + 4}}{\frac{4}{9}}
        =
        \frac{2}{9} \frac{9}{4}
        =
        \frac{1}{2}
    \end{multline*}

    \begin{multline*}
        P(X = \mathrm{fair} \mid Y = \mathrm{tail})
        =
        \frac{P(X = \mathrm{fair}, Y = \mathrm{tail})}{P(Y = \mathrm{tail})}
        =
        \frac{P(Y = \mathrm{tail} \mid X = \mathrm{fair}) P(X = \mathrm{fair})}{P(Y = \mathrm{tail})} \\
        =
        \frac{\frac{1}{2} \frac{4}{3 + 2 + 4}}{\frac{4}{9}}
        =
        \frac{2}{9} \frac{9}{4}
        =
        \frac{1}{2}
    \end{multline*}

    \item

    \begin{align*}
        &
        P(Y_2 = \mathrm{tail} \mid Y_1 = \mathrm{tail}) P(Y_1 = \mathrm{tail}) \\
        & =
        P(Y_1 = Y_2 = \mathrm{tail}) \\
        & =
        P(Y_1 = Y_2 = \mathrm{tail} \mid X_1 = \mathrm{head}, X_2 = \mathrm{head}) P(X_1 = \mathrm{head}, X_2 = \mathrm{head}) \\
        & +
        P(Y_1 = Y_2 = \mathrm{tail} \mid X_1 = \mathrm{head}, X_2 = \mathrm{tail}) P(X_1 = \mathrm{head}, X_2 = \mathrm{tail}) \\
        & +
        P(Y_1 = Y_2 = \mathrm{tail} \mid X_1 = \mathrm{head}, X_2 = \mathrm{fair}) P(X_1 = \mathrm{head}, X_2 = \mathrm{head}) \\
        & +
        P(Y_1 = Y_2 = \mathrm{tail} \mid X_1 = \mathrm{tail}, X_2 = \mathrm{head}) P(X_1 = \mathrm{tail}, X_2 = \mathrm{head}) \\
        & +
        P(Y_1 = Y_2 = \mathrm{tail} \mid X_1 = \mathrm{tail}, X_2 = \mathrm{tail}) P(X_1 = \mathrm{tail}, X_2 = \mathrm{tail}) \\
        & +
        P(Y_1 = Y_2 = \mathrm{tail} \mid X_1 = \mathrm{tail}, X_2 = \mathrm{fair}) P(X_1 = \mathrm{tail}, X_2 = \mathrm{fair}) \\
        & +
        P(Y_1 = Y_2 = \mathrm{tail} \mid X_1 = \mathrm{fair}, X_2 = \mathrm{head}) P(X_1 = \mathrm{fair}, X_2 = \mathrm{head}) \\
        & +
        P(Y_1 = Y_2 = \mathrm{tail} \mid X_1 = \mathrm{fair}, X_2 = \mathrm{tail}) P(X_1 = \mathrm{fair}, X_2 = \mathrm{tail}) \\
        & +
        P(Y_1 = Y_2 = \mathrm{tail} \mid X_1 = \mathrm{fair}, X_2 = \mathrm{fair}) P(X_1 = \mathrm{fair}, X_2 = \mathrm{fair}) \\
        & =
        P(Y_1 = Y_2 = \mathrm{tail} \mid X_1 = \mathrm{head}, X_2 = \mathrm{head}) P(X_1 = \mathrm{head}) P(X_2 = \mathrm{head} \mid X_1 = \mathrm{head}) \\
        & +
        P(Y_1 = Y_2 = \mathrm{tail} \mid X_1 = \mathrm{head}, X_2 = \mathrm{tail}) P(X_1 = \mathrm{head}) P(X_2 = \mathrm{tail} \mid X_1 = \mathrm{head}) \\
        & +
        P(Y_1 = Y_2 = \mathrm{tail} \mid X_1 = \mathrm{head}, X_2 = \mathrm{fair}) P(X_1 = \mathrm{head}) P(X_2 = \mathrm{head} \mid X_1 = \mathrm{head}) \\
        & +
        P(Y_1 = Y_2 = \mathrm{tail} \mid X_1 = \mathrm{tail}, X_2 = \mathrm{head}) P(X_1 = \mathrm{tail}) P(X_2 = \mathrm{head} \mid X_1 = \mathrm{tail}) \\
        & +
        P(Y_1 = Y_2 = \mathrm{tail} \mid X_1 = \mathrm{tail}, X_2 = \mathrm{tail}) P(X_1 = \mathrm{tail}) P(X_2 = \mathrm{tail} \mid X_1 = \mathrm{tail}) \\
        & +
        P(Y_1 = Y_2 = \mathrm{tail} \mid X_1 = \mathrm{tail}, X_2 = \mathrm{fair}) P(X_1 = \mathrm{tail}) P(X_2 = \mathrm{fair} \mid X_1 = \mathrm{tail}) \\
        & +
        P(Y_1 = Y_2 = \mathrm{tail} \mid X_1 = \mathrm{fair}, X_2 = \mathrm{head}) P(X_1 = \mathrm{fair}) P(X_2 = \mathrm{head} \mid X_1 = \mathrm{fair}) \\
        & +
        P(Y_1 = Y_2 = \mathrm{tail} \mid X_1 = \mathrm{fair}, X_2 = \mathrm{tail}) P(X_1 = \mathrm{fair}) P(X_2 = \mathrm{tail} \mid X_1 = \mathrm{fair}) \\
        & +
        P(Y_1 = Y_2 = \mathrm{tail} \mid X_1 = \mathrm{fair}, X_2 = \mathrm{fair}) P(X_1 = \mathrm{fair}) P(X_2 = \mathrm{fair} \mid X_1 = \mathrm{fair}) \\
        & =
        0           \cdot 0           \cdot \frac{3}{9} \cdot \frac{3 - 1}{8}
        +
        0           \cdot 1           \cdot \frac{3}{9} \cdot \frac{2}{8}
        +
        0           \cdot \frac{1}{2} \cdot \frac{3}{9} \cdot \frac{4}{8} \\
        & +
        1           \cdot 0           \cdot \frac{2}{9} \cdot \frac{3}{8}
        +
        1           \cdot 1           \cdot \frac{2}{9} \cdot \frac{2 - 1}{8}
        +
        1           \cdot \frac{1}{2} \cdot \frac{2}{9} \cdot \frac{4}{8} \\
        & +
        \frac{1}{2} \cdot 0           \cdot \frac{4}{9} \cdot \frac{3}{8}
        +
        \frac{1}{2} \cdot 1           \cdot \frac{4}{9} \cdot \frac{2}{8}
        +
        \frac{1}{2} \cdot \frac{1}{2} \cdot \frac{4}{9} \cdot \frac{4 - 1}{8}
    \end{align*}

\end{enumerate}

\end{solution}

% --------------------------------------------------------------------------------
