\begin{align*}
    \epsilon_h^{(1)}(g_1)
    & = \vbraces
        {
            Q(g_1) - Q_h^{(1)}(g_1)
        }
    =   \vbraces
        {
            \sum_{i=0}^{n-1} Q(g_1|_{[hi, h(i+1)]}) -
            \sum_{i=0}^{n-1} Q^{(1)}(g_1|_{[hi, h(i+1)]})
        } \\
    & \leq
        \sum_{i=0}^{n-1} \vbraces
        {
            Q(g_1|_{[hi, h(i+1)]}) -
            Q^{(1)}(g_1|_{[hi, h(i+1)]})
        }
    =   \epsilon_h^{(1)}(g_1|_{[0, h]}) +
        \sum_{i=1}^{n-1} \epsilon_h^{(1)}(g_1|_{[hi, h(i+1)]}) \\
    & \leq
        \frac{1}{6} \sqrt{h}^3 +
        \sum_{i=1}^{n-1} \frac{\sqrt{h}^3}{48 \sqrt{i}^3}
    =   \underbrace
        {
            \frac{1}{6}
            \pbraces
            {
                1 + \frac{1}{8} \sum_{i=1}^{n-1} \frac{1}{i^\frac{3}{2}}
            }
        }_{ =: \, C}
        \sqrt{h}^3
\end{align*}