% --------------------------------------------------------------------------------

\begin{exercise}

Berechnen Sie die Faltung $f \ast g$ der Funktionen

\begin{align*}
    f(x)
    & =
    \begin{cases}
        2 x & 0 \leq x \leq 2 \\
        0   & \text{sonst}
    \end{cases} \\
    g(x)
    & =
    \begin{cases}
        3 - 3 x & 1 < x < 3 \\
        0       & \text{sonst}
    \end{cases}.
\end{align*}

\end{exercise}

% --------------------------------------------------------------------------------

\begin{solution}

\phantom{}

\begin{align*}
    (f \ast g)(x)
    :=
    \Int[\R]
    {
        f(x - y) g(y)
    }{\lambda(y)}
    =
    \cdots
\end{align*}

\begin{align*}
    f(x - y) \neq 0
    & \iff
    0 \leq x - y \leq 2
    \iff
    x - 2 \leq y \leq x \\
    g(y) \neq 0
    & \iff
    1 < y < 3 \\
    & \implies
    \Bbraces{y \in \R: f(x - y) g(y) \neq 0}
    =
    [x - 2, x] \cap (1, 3)
    =:
    M_x
\end{align*}

\begin{enumerate}[label = \arabic*.]

    \item Fall ($x \leq 1$):
    
    \begin{align*}
        & \implies
        M_x = \emptyset \\
        & \implies
        \cdots = 0
    \end{align*}

    \item Fall ($1 < x < 3$):

    \begin{align*}
        & \implies
        M_x = (1, x] \neq \emptyset \\
        & \implies
        \cdots = \Int[1][x]{2 (x - y) (3 - 3 y)}{y} = -(x - 1)^3
    \end{align*}

    \item Fall ($3 \leq x < 5$):

    \begin{align*}
        & \implies
        1 \leq x - 2 < 3 \\
        & \implies
        M_x = [x - 2, 3) \setminus \Bbraces{1} \\
        & \implies
        \cdots = \Int[x-2][3]{2 (x - y) (3 - 3 y)}{y} = x^3 - 3 x^2 - 21 x + 55
    \end{align*}

    \item Fall ($5 \leq x$):

    \begin{align*}
        & \implies
        3 \leq x - 2 \\
        & \implies
        M_x = \emptyset \\
        & \implies
        \cdots = 0
    \end{align*}

\end{enumerate}

\end{solution}

% --------------------------------------------------------------------------------
