\begin{align*}
    & Q_h^{(4)}(f) \\
    & = \sum_{i=1}^n Q^{(4)}(f|_{[x_{i-1}, x_i]}) \\
    & = \sum_{i=1}^n
        \frac{x_i - x_{i-1}}{90}
        \pbraces
        {
            7  f(x_{i-1}) + 
            32 f \pbraces{\frac{3 x_{i-1} + x_i}{4}} +
            12 f \pbraces{\frac{x_{i-1} + x_i}{2}} +
            32 f \pbraces{\frac{x_{i-1} + 3 x_i}{4}} +
            7  f(x_i)
        } \\
    & = \frac{h}{90}
        \pbraces
        {
            7  \sum_{i=1}^n f(x_{i-1}) + 
            32 \sum_{i=1}^n f \pbraces{\frac{3 x_{i-1} + x_i}{4}} +
            12 \sum_{i=1}^n f \pbraces{\frac{x_{i-1} + x_i}{2}} +
            32 \sum_{i=1}^n f \pbraces{\frac{x_{i-1} + 3 x_i}{4}} +
            7  \sum_{i=1}^n f(x_i)
        } \\
    & = \frac{1}{15}
        \Bigg (
            \frac{7h}{6}
            \pbraces
            {
                  \sum_{i=1}^n f(x_{i-1}) +
                4 \sum_{i=1}^n f \pbraces{\frac{x_{i-1} + x_i}{2}} +
                  \sum_{i=1}^n f(x_i)
            } \\
    & +
            \frac{h}{6}
            \pbraces
            {
                32 \sum_{i=1}^n f \pbraces{\frac{3 x_{i-1} + x_i}{4}} -
                16 \sum_{i=1}^n f \pbraces{\frac{x_{i-1} + x_i}{2}} +
                32 \sum_{i=1}^n f \pbraces{\frac{x_{i-1} + 3 x_i}{4}}
            }
        \Bigg ) \\
    & = \frac{1}{15}
        \Bigg (
            7 Q_h^{(2)}(f) \\
    & +
            \frac{h}{6}
            \pbraces
            {
                32 \sum_{i=1}^n f \pbraces{\frac{3 x_{i-1} + x_i}{4}} -
                16 \sum_{i=1}^n f \pbraces{\frac{x_{i-1} + x_i}{2}} +
                32 \sum_{i=1}^n f \pbraces{\frac{x_{i-1} + 3 x_i}{4}}
            }
        \Bigg )
\end{align*}

\begin{align*}
    & Q_h^{(4)}(f) \\
    & = \frac{1}{15}
        \Bigg (
            \frac{h}{6}
            \pbraces
            {
                f(a) +
                4 \sum_{i=1}^n f \pbraces{\frac{x_{i-1} + x_i}{2}} +
                2 \sum_{i=1}^{n-1} f(x_i) +
                f(b)
            } \\
    & +
            \frac{h}{6}
            \pbraces
            {
                32 \sum_{i=1}^n f \pbraces{\frac{3 x_{i-1} + x_i}{4}} -
                16 \sum_{i=1}^n f \pbraces{\frac{x_{i-1} + x_i}{2}} +
                32 \sum_{i=1}^n f \pbraces{\frac{x_{i-1} + 3 x_i}{4}}
            }
        \Bigg ) \\
    & = \frac{h}{90}
        \pbraces
        {
            7 f(a) +
            32 \sum_{i=1}^n f \pbraces{\frac{3 x_{i-1} + x_i}{4}} +
            12 \sum_{i=1}^n f \pbraces{\frac{x_{i-1} + x_i}{2}} +
            14 \sum_{i=1}^{n-1} f(x_i) +
            32 \sum_{i=1}^n f \pbraces{\frac{x_{i-1} + 3 x_i}{4}} +
            7 f(b)
        }
\end{align*}